high2/Zeta.High.Interleave.fsti
@@ -44,8 +44,9 @@ val eac_boundary (#app #n:_) (il: neac_log app n)
   : (i: seq_index il{is_eac (prefix il i) /\
                      ~ (is_eac (prefix il (i+1)))})
 
-val lemma_eac_implies_prefix_eac (#app #n:_) (il: eac_log app n) (i: nat{i <= S.length il})
-  : Lemma (ensures (is_eac (prefix il i)))
+val lemma_eac_implies_prefix_eac (#app #n:_) (il: verifiable_log app n) (i: nat{i <= S.length il})
+  : Lemma (ensures (is_eac il ==> is_eac (prefix il i)))
+          [SMTPat (prefix il i)]
 
 val lemma_eac_implies_appfn_calls_seq_consistent (#app #n:_) (il: eac_log app n)
   : Lemma (ensures (let gl = to_glog il in
