high2/Zeta.High.TSLog.fsti
@@ -2,10 +2,12 @@ module Zeta.High.TSLog
 
 open Zeta.App
 open Zeta.Time
+open Zeta.Generic.Interleave
 open Zeta.Generic.TSLog
 open Zeta.High.Verifier
 open Zeta.High.Interleave
 
+module S = FStar.Seq
 module T = Zeta.Generic.TSLog
 
 let its_log (app: app_params)
@@ -13,3 +15,7 @@ let its_log (app: app_params)
 
 let neac_before_epoch (app n:_) (ep: epoch)
   = itsl: its_log app n {not (is_eac (prefix_within_epoch ep itsl))}
+
+val neac_before_epoch_implies_neac (#app #n:_) (ep: epoch) (itsl: neac_before_epoch app n ep)
+  : Lemma (ensures (not (is_eac itsl)))
+          [SMTPat (prefix_within_epoch ep itsl)]
